Añadidos lemas

Especificaciones/VertexCoverOpt.dfy
@@ -2,7 +2,8 @@ include "VertexCover.dfy"
 //predicado de PCV
 ghost predicate optimalValueVertexCover (graph : Graph, k : nat) 
     requires isValidGraph(graph) 
-{     VertexCover(graph, k) 
+{     
+    VertexCover(graph, k) 
    && forall x : nat |  x <= |graph.0| && VertexCover(graph, x) :: x >= k
 } 
 //In this definition the bound x <= |graph.0| does not constraint anything
@@ -14,7 +15,7 @@ ghost predicate optimalValueVertexCover (graph : Graph, k : nat)
 //Optimal value vertex cover will never be strictly higher than |graph.0|
 //because VertexCover(graph, |graph.0|) always holds
 
-lemma boundoptimalValueVertexCover(graph : Graph, k : nat) 
+lemma boundoptimalValueVertexCover(graph: Graph, k : nat) 
 requires isValidGraph(graph)
 requires optimalValueVertexCover(graph,k)
 ensures k <= |graph.0|
@@ -22,19 +23,41 @@ ensures k <= |graph.0|
     assert VertexCover(graph,|graph.0|);
 }
 
+lemma emptyOptimalValueVertexCover(graph: Graph) 
+requires isValidGraph(graph)
+ensures graph.1 == {} ==> optimalValueVertexCover(graph, 0)
+{
+    assert graph.1 == {} ==> isVertexCover({}, graph);
+}
+
 //POCV predicate 
 //S to denote sets
-ghost predicate optimalVertexCover (graph : Graph, I : set<Node>)
+ghost predicate optimalVertexCover (graph: Graph, I : set<Node>)
     requires isValidGraph(graph) 
 {
        I <= graph.0 
     && isVertexCover(I, graph) 
-    && forall S | S <= graph.0 && isVertexCover(S, graph) :: |S| >= |I|
+    && forall S: set<Node> | S <= graph.0 && isVertexCover(S, graph) :: |S| >= |I|
 }
 
-lemma boundoptimalVertexCover(graph : Graph, I : set<Node>) 
+lemma boundoptimalVertexCover(graph: Graph, I : set<Node>) 
 requires isValidGraph(graph)
 requires optimalVertexCover(graph,I)
 ensures |I| <= |graph.0|
 ensures optimalValueVertexCover(graph,|I|)
 {  }
+
+lemma translationVertexCover(graph: Graph, k: nat) 
+requires isValidGraph(graph)
+requires optimalValueVertexCover(graph, k)
+ensures exists I: set<Node> :: I <= graph.0 && optimalVertexCover(graph, I) && |I| == k
+ensures !exists I:set<Node> | I <= graph.0 && |I| < k  :: isVertexCover(I,graph)
+{
+    if exists I:set<Node> :: I <= graph.0 && |I| < k && isVertexCover(I,graph)
+    {
+        ghost var I: set<Node> :| I <= graph.0 && |I| < k && isVertexCover(I,graph);
+        assert VertexCover(graph, |I|);
+        cardinalityLemma3(I, graph.0);
+        assert false;
+    }
+}
